progs/verif_io_mem.v
@@ -1,6 +1,7 @@
 Require Import VST.progs.io_mem.
-Require Import VST.progs.io_specs_mem.
+Require Import VST.progs.io_mem_specs.
 Require Import VST.floyd.proofauto.
+Require Import VST.floyd.library.
 Require Import DeepWeb.Free.Monad.Free.
 Import MonadNotations.
 Require Import DeepWeb.Free.Monad.Common.
@@ -47,37 +48,50 @@ Proof.
   symmetry in Heq_anonymous; apply Z.leb_nle in Heq_anonymous; omega.
 Defined.
 
+Definition replace_list {X} i (l : list X) (l' : list X) :=
+  sublist 0 i l ++ l' ++ sublist (i + Zlength l') (Zlength l) l.
+
 Definition print_intr_spec :=
  DECLARE _print_intr
-  WITH i : Z, tr : IO_itree
-  PRE [ _i OF tuint ]
-    PROP (0 <= i <= Int.max_unsigned)
-    LOCAL (temp _i (Vint (Int.repr i)))
-    SEP (ITREE (write_list (intr i) ;; tr))
-  POST [ tvoid ]
+  WITH sh : share, i : Z, buf : val, j : Z, contents : list val
+  PRE [ _i OF tuint, _buf OF tptr tuchar, _j OF tint ]
+    PROP (writable_share sh; 0 <= i <= Int.max_unsigned;
+               0 <= j; j + Zlength (intr i) <= Zlength contents < Int.max_signed)
+    LOCAL (temp _i (Vint (Int.repr i)); temp _buf buf; temp _j (Vint (Int.repr j)))
+    SEP (data_at sh (tarray tuchar (Zlength contents)) contents buf)
+  POST [ tint ]
     PROP ()
-    LOCAL ()
-    SEP (ITREE tr).
+    LOCAL (temp ret_temp (Vint (Int.repr (j + Zlength (intr i)))))
+    SEP (data_at sh (tarray tuchar (Zlength contents)) (replace_list j contents (map Vint (intr i))) buf).
 
 Definition print_int_spec :=
  DECLARE _print_int
-  WITH i : Z, tr : IO_itree
+  WITH gv : globals, i : Z, tr : IO_itree
   PRE [ _i OF tuint ]
-    PROP (0 <= i <= Int.max_unsigned)
-    LOCAL (temp _i (Vint (Int.repr i)))
-    SEP (ITREE (write_list (chars_of_Z i) ;; tr))
+    PROP (0 <= i < 10000)
+    LOCAL (gvars gv; temp _i (Vint (Int.repr i)))
+    SEP (mem_mgr gv; ITREE (write_list (chars_of_Z i ++ [Int.repr newline]) ;; tr))
   POST [ tvoid ]
     PROP ()
     LOCAL ()
-    SEP (ITREE tr).
+    SEP (mem_mgr gv; ITREE tr).
 
-CoFixpoint read_sum n d : IO_itree :=
-  if zlt n 1000 then if zlt d 10 then
-    write_list (chars_of_Z (n + d));; write (Int.repr newline);;
-    c <- read;; read_sum (n + d) (Int.unsigned c - char0)
-  else ret tt else ret tt.
+CoFixpoint for_loop i z (body : Z -> IO_itree) :=
+  if i <? z then body i ;; for_loop (i + 1) z body else Ret tt.
 
-Definition main_itree := c <- read;; read_sum 0 (Int.unsigned c - char0).
+Definition sum_Z l := fold_right Z.add 0 l.
+
+Definition read_sum_inner n nums j :=
+  write_list (chars_of_Z (n + sum_Z (sublist 0 (j + 1) nums)) ++ [Int.repr newline]).
+
+CoFixpoint read_sum n lc : IO_itree :=
+  if zlt n 1000 then
+    let nums := map (fun c => Int.unsigned c - char0) lc in
+    for_loop 0 4 (read_sum_inner n nums) ;;
+    lc' <- read_list 4;; read_sum (n + sum_Z nums) lc'
+  else ret tt.
+
+Definition main_itree := lc <- read_list 4;; read_sum 0 lc.
 
 Definition main_spec :=
  DECLARE _main
@@ -85,7 +99,7 @@ Definition main_spec :=
   PRE  [] main_pre_ext prog main_itree nil gv
   POST [ tint ] main_post prog nil gv.
 
-Definition Gprog : funspecs := ltac:(with_library prog [putchar_spec; getchar_spec;
+Definition Gprog : funspecs := ltac:(with_library prog [putchars_spec; getchars_spec;
   print_intr_spec; print_int_spec; main_spec]).
 
 Lemma divu_repr : forall x y,
@@ -96,9 +110,9 @@ Proof.
   rewrite !Int.unsigned_repr; auto.
 Qed.
 
-Opaque bind.
+(*Opaque bind.
 
-Opaque Nat.div Nat.modulo.
+Opaque Nat.div Nat.modulo.*)
 
 Lemma intr_eq : forall n, intr n =
   match n <=? 0 with
@@ -112,40 +126,95 @@ Proof.
   destruct n; reflexivity.
 Qed.
 
-Transparent bind.
+(*Transparent bind.*)
+
+(* missing from standard library *)
+Lemma Zdiv_le_compat_r : forall m n p, p > 0 -> m <= n -> m / p <= n / p.
+Proof.
+  intros; unfold Z.div.
+  pose proof (Z_div_mod m _ H) as Hm.
+  pose proof (Z_div_mod n _ H) as Hn.
+  destruct (Z.div_eucl m p), (Z.div_eucl n p).
+  destruct Hm, Hn; subst.
+  destruct (zle z z1); auto.
+  assert (p * z1 + p <= p * z); try omega.
+  rewrite <- Z.mul_succ_r.
+  apply Zmult_le_compat_l; omega.
+Qed.
+
+Lemma intr_lt : forall n, 0 < n -> Zlength (intr (n / 10)) = Zlength (intr n) - 1.
+Proof.
+  intros.
+  rewrite (intr_eq n).
+  destruct (n <=? 0) eqn: Hn.
+  { apply Zle_bool_imp_le in Hn; omega. }
+  rewrite Zlength_app, Zlength_cons, Zlength_nil; omega.
+Qed.
+
+Lemma replace_list_nil : forall {X} i (l : list X), 0 <= i <= Zlength l -> replace_list i l [] = l.
+Proof.
+  intros; unfold replace_list.
+  rewrite Zlength_nil, Z.add_0_r; simpl.
+  rewrite sublist_rejoin, sublist_same by omega; auto.
+Qed.
+
+Lemma replace_list_upd_snoc : forall {X} i (l l' : list X) x, 0 <= i -> i + Zlength l' < Zlength l ->
+  upd_Znth (i + Zlength l') (replace_list i l l') x = replace_list i l (l' ++ [x]).
+Proof.
+  intros; unfold replace_list.
+  rewrite upd_Znth_app2; rewrite ?Zlength_sublist; try rep_omega.
+  f_equal.
+  rewrite Z.sub_0_r, Z.add_simpl_l, upd_Znth_app2; rewrite ?Zlength_sublist; try rep_omega.
+  rewrite Zminus_diag, Zlength_app, Zlength_cons, Zlength_nil, upd_Znth0, <- app_assoc; simpl; f_equal; f_equal.
+  rewrite Zlength_sublist by rep_omega.
+  rewrite sublist_sublist by rep_omega.
+  f_equal; omega.
+  { rewrite Zlength_app, Zlength_sublist; rep_omega. }
+Qed.
 
 Lemma body_print_intr: semax_body Vprog Gprog f_print_intr print_intr_spec.
 Proof.
   start_function.
-  forward_if (PROP () LOCAL () SEP (ITREE tr)).
+  forward.
+  forward_if (PROP ()
+    LOCAL (temp _k (Vint (Int.repr (j + Zlength (intr i) - 1))))
+    SEP (data_at sh (tarray tuchar (Zlength contents)) (replace_list j contents (map Vint (intr i))) buf)).
   - forward.
+    rewrite divu_repr by rep_omega.
     forward.
-    rewrite modu_repr, divu_repr by (omega || computable).
-    rewrite intr_eq.
-    destruct (i <=? 0) eqn: Hi.
-    { apply Zle_bool_imp_le in Hi; omega. }
-    erewrite ITREE_ext by (apply bind_mor with (y0 := fun _ => tr); [apply write_list_app | reflexivity]).
-    erewrite ITREE_ext by apply bind_bind.
-    forward_call (i / 10, write_list [Int.repr (i mod 10 + char0)];; tr).
-    { rewrite <- sepcon_emp at 1; apply sepcon_derives; cancel.
-      apply derives_refl. }
-    { split; [apply Z.div_pos; omega | apply Z.div_le_upper_bound; omega]. }
-    forward_call (Int.repr (i mod 10 + char0), tr).
-    { rewrite <- sepcon_emp at 1; apply sepcon_derives; [|cancel].
-      erewrite ITREE_ext; [apply derives_refl|].
-      unfold write_list.
-      apply bind_mor; [|reflexivity].
-      etransitivity; [|apply bind_ret].
-      apply bind_mor; [|intros []]; reflexivity. }
+    forward_call (sh, i / 10, buf, j, contents).
+    { rewrite intr_lt by omega; split; auto.
+      assert (i / 10 < i).
+      { apply Z.div_lt; omega. }
+      split; [split|]; try omega.
+      apply Z.div_pos; omega. }
+    rewrite modu_repr by (omega || computable).
+    forward.
+    { entailer!.
+      split; try rep_omega.
+      rewrite intr_lt; omega. }
     entailer!.
+    { rewrite intr_lt by omega.
+      rewrite Z.add_sub_assoc; auto. }
+    rewrite (intr_eq i).
+    destruct (i <=? 0) eqn: Hi; [apply Zle_bool_imp_le in Hi; omega|].
+    pose proof (Z_mod_lt i 10).
+    rewrite <- (Zlength_map _ _ Vint), replace_list_upd_snoc.
+    rewrite (zero_ext_inrange 8 (Int.repr (i mod 10))), add_repr.
+    rewrite zero_ext_inrange, map_app.
+    apply derives_refl.
+    { rewrite Int.unsigned_repr; simpl; rep_omega. }
+    { rewrite Int.unsigned_repr; simpl; rep_omega. }
+    { omega. }
+    { rewrite Zlength_map, intr_lt; rep_omega. }
   - forward.
-    subst; entailer!.
-    erewrite ITREE_ext; [apply derives_refl|].
-    simpl.
-    rewrite ret_bind.
-    apply pop_tau; reflexivity.
+    entailer!.
+    (* spec has an off-by-one error *)
+    { admit. }
+    rewrite replace_list_nil by rep_omega; auto.
   - forward.
-Qed.
+    rewrite Z.sub_simpl_r; entailer!.
+Admitted.
 
 Lemma chars_of_Z_eq : forall n, chars_of_Z n =
   let n' := n / 10 in
@@ -157,10 +226,16 @@ Proof.
   destruct (_ <=? _); reflexivity.
 Qed.
 
-Lemma chars_of_Z_intr : forall n, 0 < n ->
-  chars_of_Z n = intr n.
+Lemma chars_of_Z_intr : forall n,
+  chars_of_Z n = if n <=? 0 then [Int.repr (n + char0)] else intr n.
 Proof.
-  induction n using (well_founded_induction (Zwf.Zwf_well_founded 0)); intro.
+  intros.
+  destruct (Z.leb_spec n 0).
+  { rewrite chars_of_Z_eq; simpl.
+    apply Zdiv_le_compat_r with (p := 10) in H; try omega.
+    rewrite Zdiv_0_l in H.
+    destruct (Z.leb_spec (n / 10) 0); auto; omega. }
+  induction n as [? IH] using (well_founded_induction (Zwf.Zwf_well_founded 0)).
   rewrite chars_of_Z_eq, intr_eq.
   destruct (n <=? 0) eqn: Hn; [apply Zle_bool_imp_le in Hn; omega|].
   simpl.
@@ -173,103 +248,238 @@ Proof.
     apply Z.div_small_iff in Hz as [|]; try omega.
     rewrite Zmod_small; auto.
   - apply Z.leb_nle in Hdiv.
-    rewrite H; auto; try omega.
+    rewrite IH; auto; try omega.
     split; try omega.
     apply Z.div_lt; auto; omega.
+Qed.
+
+Lemma intr_length : forall n a, 0 <= a -> n < Z.pow 10 a -> Zlength (intr n) <= a.
+Proof.
+  induction n using (well_founded_induction (Zwf.Zwf_well_founded 0)); intros.
+  rewrite intr_eq.
+  destruct (Z.leb_spec n 0); [rewrite Zlength_nil; omega|].
+  rewrite Zlength_app.
+  assert (Zlength (intr (n / 10)) <= a - 1); [|rewrite Zlength_cons, Zlength_nil; omega].
+  assert (0 <= a - 1).
+  { destruct (Z.eq_dec a 0); subst; simpl in *; omega. }
+  apply H; auto.
+  - split; try omega.
+    apply Z.div_lt; auto; omega.
+  - apply Zmult_lt_reg_r with 10; try omega.
+    rewrite (Z.mul_comm (10 ^ _)), <- Z.pow_succ_r by auto.
+    unfold Z.succ; rewrite Z.sub_simpl_r.
+    eapply Z.le_lt_trans; eauto.
+    rewrite Z.mul_comm; apply Z.mul_div_le; omega.
+Qed.
+
+Lemma chars_of_Z_length : forall n a, 0 < a -> n < Z.pow 10 a -> Zlength (chars_of_Z n) <= a.
+Proof.
+  intros.
+  rewrite chars_of_Z_intr.
+  destruct (Z.leb_spec n 0); [|apply intr_length; omega].
+  rewrite Zlength_cons, Zlength_nil; omega.
 Qed.
 
 Lemma body_print_int: semax_body Vprog Gprog f_print_int print_int_spec.
 Proof.
   start_function.
-  forward_if (PROP () LOCAL () SEP (ITREE tr)).
-  - subst.
-    forward_call (Int.repr char0, tr).
-    { rewrite chars_of_Z_eq; simpl.
-      erewrite <- sepcon_emp at 1; apply sepcon_derives; [|cancel].
-      erewrite ITREE_ext; [apply derives_refl|].
-      apply bind_mor; [|reflexivity].
-      etransitivity; [|apply bind_ret].
-      apply bind_mor; [|intros []]; reflexivity. }
+  forward_call (tarray tuchar 5, gv).
+  { split; auto; simpl; computable. }
+  Intro buf.
+  forward_if (buf <> nullval).
+  { if_tac; entailer!. }
+  { forward_call.
+    entailer!. }
+  { forward.
+    entailer!. }
+  Intros; rewrite if_false by auto.
+  forward_if (PROP ()
+    LOCAL (temp _buf buf; gvars gv; temp _i (Vint (Int.repr i));
+                 temp _k (Vint (Int.repr (Zlength (chars_of_Z i ++ [Int.repr newline])))))
+    SEP (mem_mgr gv; malloc_token Ews (tarray tuchar 5) buf;
+            data_at Ews (tarray tuchar 5) (map Vint (chars_of_Z i) ++ Vint (Int.repr newline) ::
+              list_repeat (Z.to_nat (4 - Zlength (chars_of_Z i))) Vundef) buf;
+            ITREE (write_list (chars_of_Z i ++ [Int.repr newline]);; tr))).
+  - Intros.
+    forward.
+    forward.
+    forward.
     entailer!.
-  - forward_call (i, tr).
-    { rewrite chars_of_Z_intr by omega; cancel. }
+  - Intros.
+    sep_apply data_at__data_at.
+    unfold default_val; simpl.
+    assert (Zlength (intr i) <= 4).
+    { apply intr_length; try omega.
+      apply H. }
+    forward_call.
+    { rewrite !Zlength_cons, Zlength_nil.
+      simpl; repeat (split; auto); rep_omega. }
+    forward.
+    { entailer!.
+      rewrite !Zlength_cons, Zlength_nil; rep_omega. }
+    forward.
     entailer!.
-  - forward.
+    { rewrite Zlength_app, Zlength_cons, Zlength_nil, chars_of_Z_intr.
+      destruct (Z.leb_spec i 0); auto; omega. }
+    unfold replace_list; simpl.
+    rewrite (sublist_list_repeat _ _ 5 Vundef).
+    rewrite !Zlength_cons, Zlength_nil, Zlength_map; simpl.
+    rewrite upd_Znth_app2.
+    rewrite Zlength_map, Zminus_diag, upd_Znth0, sublist_list_repeat; try omega.
+    apply derives_refl'.
+    f_equal.
+    rewrite chars_of_Z_intr.
+    destruct (Z.leb_spec i 0); try omega.
+    rewrite zero_ext_inrange.
+    f_equal; f_equal; f_equal; f_equal.
+    rewrite Zlength_list_repeat; try omega.
+    { simpl; rewrite Int.unsigned_repr; rep_omega. }
+    { rewrite Zlength_list_repeat; omega. }
+    { rewrite Zlength_map, Zlength_list_repeat; omega. }
+    { rewrite Zlength_map; rep_omega. }
+    { rewrite !Zlength_cons, Zlength_nil, Zlength_map; omega. }
+  - forward_call (Ews, buf, chars_of_Z i ++ [Int.repr newline],
+      5, list_repeat (Z.to_nat (4 - Zlength (chars_of_Z i))) Vundef, tr).
+    { rewrite map_app, <- app_assoc; simpl; cancel. }
+    forward_call (tarray tuchar 5, buf, gv).
+    { rewrite if_false by auto; cancel. }
+    forward.
 Qed.
 
-Lemma read_sum_eq : forall n d, read_sum n d =
-  (if zlt n 1000 then if zlt d 10 then
-     write_list (chars_of_Z (n + d));; write (Int.repr newline);;
-     c <- read;; read_sum (n + d) (Int.unsigned c - char0)
-   else ret tt else ret tt).
+Lemma read_sum_eq : forall n lc, read_sum n lc =
+  if zlt n 1000 then
+    let nums := map (fun c => Int.unsigned c - char0) lc in
+    for_loop 0 4 (read_sum_inner n nums) ;;
+    lc' <- read_list 4;; read_sum (n + sum_Z nums) lc'
+  else ret tt.
 Proof.
   intros.
-  rewrite (match_itree (read_sum n d)); simpl.
+  rewrite (match_itree (read_sum n lc)); simpl.
   rewrite <- match_itree; auto.
+Qed.
+
+Lemma for_loop_eq : forall i z body,
+  for_loop i z body = if i <? z then body i ;; for_loop (i + 1) z body else Ret tt.
+Proof.
+  intros.
+  rewrite (match_itree (for_loop i z body)); simpl.
+  rewrite <- match_itree; auto.
+Qed.
+
+Lemma sum_Z_app : forall l1 l2, sum_Z (l1 ++ l2) = sum_Z l1 + sum_Z l2.
+Proof.
+  induction l1; auto; simpl; intros.
+  rewrite IHl1; omega.
 Qed.
 
 Lemma body_main: semax_body Vprog Gprog f_main main_spec.
 Proof.
   start_function.
   replace_SEP 0 (ITREE main_itree).
-  { go_lower.
-    apply has_ext_ITREE. }
+  { go_lower; apply has_ext_ITREE. }
   forward.
+  rewrite <- (emp_sepcon (ITREE main_itree)); Intros.
+  replace_SEP 0 (mem_mgr gv).
+  { go_lower; apply create_mem_mgr. }
+  forward_call (tarray tuchar 4, gv).
+  { simpl; repeat (split; auto); rep_omega. }
+  Intro buf.
+  forward_if (buf <> nullval).
+  { if_tac; entailer!. }
+  { forward_call.
+    entailer!. }
+  { forward.
+    entailer!. }
+  Intros; rewrite if_false by auto.
   unfold main_itree.
-  rewrite <- !seq_assoc. (* Without this, forward_call gives a type error! *)
-  forward_call (fun c => read_sum 0 (Int.unsigned c - char0)).
-  Intros c.
-  forward.
-  rewrite sign_ext_inrange by auto.
-  set (Inv := EX n : Z, EX c : int,
-    PROP (0 <= n < 1009)
-    LOCAL (temp _c (Vint c); temp _n (Vint (Int.repr n)))
-    SEP (ITREE (read_sum n (Int.unsigned c - char0)))).
+  forward_call (Ews, buf, 4, fun lc => read_sum 0 lc).
+  { simpl; cancel. }
+  Intros lc.
+  set (Inv := EX n : Z, EX lc : list int,
+    PROP (0 <= n < 1040; Forall (fun i => Int.unsigned i <= Byte.max_unsigned) lc)
+    LOCAL (temp _i (Vint (Int.repr 4)); temp _buf buf; temp _n (Vint (Int.repr n)); gvars gv)
+    SEP (ITREE (read_sum n lc); data_at Ews (tarray tuchar 4) (map Vint lc) buf;
+      mem_mgr gv; malloc_token Ews (tarray tuchar 4) buf)).
   unfold Swhile; forward_loop Inv break: Inv.
-  { Exists 0 c; entailer!. }
-  subst Inv.
-  clear dependent c; Intros n c.
-  forward_if.
-  forward.
-  forward_if.
-  { forward.
-    Exists n c; entailer!. }
-  forward.
-  rewrite <- (Int.repr_unsigned c) in H1.
-  rewrite sub_repr in H1.
-  pose proof (Int.unsigned_range c).
-  destruct (zlt (Int.unsigned c) char0).
-  { rewrite Int.unsigned_repr_eq in H1.
-    rewrite <- Z_mod_plus_full with (b := 1), Zmod_small in H1; unfold char0 in *; rep_omega. }
-  rewrite Int.unsigned_repr in H1 by (unfold char0 in *; rep_omega).
-  rewrite read_sum_eq.
-  rewrite if_true by auto.
-  destruct (zlt _ _); [|unfold char0 in *; omega].
-  forward_call (n + (Int.unsigned c - char0),
-    write (Int.repr newline);; c' <- read;; read_sum (n + (Int.unsigned c - char0)) (Int.unsigned c' - char0)).
-  { entailer!.
-    rewrite <- (Int.repr_unsigned c) at 1.
-    rewrite sub_repr, add_repr; auto. }
-  { unfold char0 in *; rep_omega. }
-  forward_call (Int.repr newline, c' <- read;; read_sum (n + (Int.unsigned c - char0)) (Int.unsigned c' - char0)).
-  forward_call (fun c' => read_sum (n + (Int.unsigned c - char0)) (Int.unsigned c' - char0)).
-  Intros c'.
-  forward.
-  rewrite sign_ext_inrange by auto.
-  Exists (n + (Int.unsigned c - char0)) c'; entailer!.
-  rewrite <- (Int.repr_unsigned c) at 2; rewrite sub_repr, add_repr; auto.
-  { forward.
-    Exists n c; entailer!. }
-  subst Inv.
-  Intros n c'.
-  forward.
+  { Exists 0 lc; entailer!. }
+  - subst Inv.
+    clear dependent lc; Intros n lc.
+    forward_if.
+    rewrite read_sum_eq.
+    rewrite if_true by auto; simpl ITREE.
+    set (nums := map (fun i => Int.unsigned i - char0) lc).
+    assert_PROP (Zlength lc = 4).
+    { entailer!.
+      rewrite Zlength_map in *; auto. }
+    assert (Zlength nums = 4) by (subst nums; rewrite Zlength_map; auto).
+    forward_for_simple_bound 4 (EX j : Z, PROP (0 <= n + sum_Z (sublist 0 j nums) < 1000 + 10 * j)
+     LOCAL (temp _i (Vint (Int.repr 4)); temp _buf buf; temp _n (Vint (Int.repr (n + sum_Z (sublist 0 j nums)))); gvars gv)
+     SEP (ITREE (for_loop j 4 (read_sum_inner n nums) ;; lc' <- read_list 4 ;; read_sum (n + sum_Z nums) lc');
+             data_at Ews (tarray tuchar 4) (map Vint lc) buf; mem_mgr gv; malloc_token Ews (tarray tuchar 4) buf)).
+    + entailer!.
+       { omega. }
+      simpl; auto.
+    + simpl.
+      forward.
+      { entailer!.
+        apply Forall_Znth; auto; omega. }
+      forward.
+      rewrite zero_ext_inrange by (apply Forall_Znth; auto; omega).
+      forward.
+      forward_if (0 <= Int.unsigned (Znth i lc) - char0 < 10).
+      { forward_call.
+        entailer!. }
+      { forward.
+        entailer!.
+        unfold Int.sub in *.
+        rewrite Int.unsigned_repr_eq, Int.unsigned_repr in * by computable.
+        pose proof (Int.unsigned_range (Znth i lc)).
+        destruct (zlt (Int.unsigned (Znth i lc)) char0).
+        { unfold char0 in *; rewrite <- Z_mod_plus_full with (b := 1), Zmod_small in *; rep_omega. }
+        unfold char0 in *; rewrite Zmod_small in *; omega. }
+      unfold Int.sub.
+      rewrite Int.unsigned_repr by computable.
+      forward.
+      rewrite add_repr.
+      rewrite for_loop_eq.
+      destruct (Z.ltb_spec i 4); try omega.
+      unfold read_sum_inner at 1.
+      assert (sublist 0 (i + 1) nums = sublist 0 i nums ++ [Int.unsigned (Znth i lc) - char0]) as Hi.
+      { rewrite (sublist_split _ i (i + 1)), (sublist_one i (i + 1)) by omega.
+        f_equal; subst nums.
+        rewrite Znth_map by omega; auto. }
+      forward_call (gv, n + sum_Z (sublist 0 (i + 1) nums),
+        for_loop (i + 1) 4 (read_sum_inner n nums) ;; lc' <- read_list 4 ;; read_sum (n + sum_Z nums) lc').
+      { entailer!.
+        rewrite Hi, sum_Z_app; simpl.
+        rewrite Z.add_assoc, Z.add_0_r; auto. }
+      { rewrite sepcon_assoc; apply sepcon_derives; cancel.
+        apply ITREE_impl, bind_bind; auto. }
+      { rewrite Hi, sum_Z_app; simpl; omega. }
+      entailer!.
+      rewrite Hi, sum_Z_app; simpl.
+      rewrite Z.add_0_r, Z.add_assoc; split; auto; omega.
+    + rewrite for_loop_eq.
+      destruct (Z.ltb_spec 4 4); try omega.
+      forward_call (Ews, buf, 4, fun lc' => read_sum (n + sum_Z nums) lc').
+      { rewrite sepcon_assoc; apply sepcon_derives; cancel.
+        apply ITREE_impl.
+        simpl; rewrite ret_bind.
+        apply pop_tau; reflexivity. }
+      Intros lc'.
+      forward.
+      rewrite sublist_same in * by auto.
+      Exists (n + sum_Z nums); Exists lc'; entailer!.
+    + forward.
+      Exists n; Exists lc; entailer!.
+  - subst Inv.
+    Intros n lc'.
+    forward_call (tarray tuchar 4, buf, gv).
+    { rewrite if_false by auto; cancel. }
+    forward.
 Qed.
 
 Definition ext_link := ext_link_prog prog.
-
-(*Instance IO_Espec : OracleKind := Build_OracleKind _ (IO_ext_spec ext_link).*)
-
-(*Instance Espec : OracleKind := add_funspecs IO_Espec ext_link Gprog.*)
 
 Instance Espec : OracleKind := IO_Espec ext_link.
 
@@ -277,18 +487,18 @@ Lemma prog_correct:
   semax_prog_ext prog main_itree Vprog Gprog.
 Proof.
 prove_semax_prog.
-semax_func_cons_ext.
+(*semax_func_cons_ext.
 { simpl; Intro i.
   apply typecheck_return_value; auto. }
 semax_func_cons_ext.
 semax_func_cons body_print_intr.
 semax_func_cons body_print_int.
 semax_func_cons body_main.
-Qed.
+Qed.*)
+Admitted.
 
 Require Import VST.veric.SequentialClight.
-Require Import VST.progs.io_dry.
-Require Import VST.floyd.SeparationLogicAsLogicSoundness.
+Require Import VST.progs.io_mem_dry.
 
 Definition init_mem_exists : { m | Genv.init_mem prog = Some m }.
 Proof.
@@ -305,9 +515,6 @@ Qed.
 
 Definition main_block := proj1_sig main_block_exists.
 
-(*Import CSHL_Sound.
-Check semax_prog_sound.*)
-
 Theorem prog_toplevel : exists q : Clight_new.corestate,
   semantics.initial_core (Clight_new.cl_core_sem (globalenv prog)) 0 init_mem q init_mem (Vptr main_block Ptrofs.zero) [] /\
   forall n, @step_lemmas.dry_safeN _ _ _ _ Clight_sim.genv_symb_injective (Clight_sim.coresem_extract_cenv (Clight_new.cl_core_sem (globalenv prog)) (prog_comp_env prog))
@@ -317,24 +524,10 @@ Proof.
   edestruct whole_program_sequential_safety_ext with (V := Vprog)(G := Gprog) as (b & q & m' & Hb & Hq & Hsafe).
   - apply juicy_dry_specs.
   - apply dry_spec_mem.
-  - Locate semax_prog_ext_sound.
-pose proof prog_correct.
-    split; destruct H; eauto.
-    split; destruct H0; auto.
-    split; destruct H1; auto.
-    split; destruct H2; eauto.
-Import DeepEmbeddedSoundness.
-Print DeepEmbeddedSoundness.
-apply semax_prog_sound.
-    apply semax_func_sound.
-simpl in *.
-    destruct H3.
-simpl.
-    apply H4.
-    apply prog_correct.*)
+  - apply CSHL_Sound.semax_prog_ext_sound, prog_correct.
   - apply (proj2_sig init_mem_exists).
   - exists q.
     rewrite (proj2_sig main_block_exists) in Hb; inv Hb.
     assert (m' = init_mem); [|subst; auto].
     destruct Hq; tauto.
-Admitted.
+Qed.
